wip

src/localdrf/LocalDRF_PF.v
@@ -108,3 +108,345 @@ Section LOCALDRF.
   Admitted.
 
 End LOCALDRF.
+
+Section SIM.
+
+  Variable L: Loc.t -> Prop.
+
+  Inductive sim_memory_content :
+    option (Time.t * Message.t) -> option (Time.t * Message.t) -> Prop :=
+  | sim_memory_content_some
+      from_tgt from_src msg_src msg_tgt
+      (FROM: Time.le from_tgt from_src)
+      (MESSAGE: Message.le msg_src msg_tgt)
+    :
+      sim_memory_content
+        (Some (from_src, msg_src))
+        (Some (from_tgt, msg_tgt))
+  | sim_memory_content_none
+    :
+      sim_memory_content None None
+  .
+
+  Inductive sim_memory P mem_src mem_tgt : Prop :=
+  | sim_memory_intro
+      (COMPLETE: forall l t (NPROMS: ~ P l t),
+          sim_memory_content
+            (Memory.get l t mem_src) (Memory.get l t mem_tgt))
+      (FORGET: forall l t (PROMS: P l t), Memory.get l t mem_src = None)
+  .
+
+  Inductive sim_memory P mem_src mem_tgt : Prop :=
+  | sim_memory_intro
+      (COMPLETE: forall l t (NPROMS: ~ P l t),
+          sim_memory_content
+            (Memory.get l t mem_src) (Memory.get l t mem_tgt))
+      (FORGET: forall l t (PROMS: P l t), Memory.get l t mem_src = None)
+  .
+
+
+  Inductive sim_promise
+
+  Inductive sim_statelocal:
+    sigT (@Language.state ProgramEvent.t) * Local.t -> sigT (@Language.state ProgramEvent.t) * Local.t -> Prop :=
+  | forget_statelocal_intro
+      st lc_src lc_tgt
+      (TVIEW : TView.le lc_src.(Local.tview) lc_tgt.(Local.tview))
+      (PROMS : lc1.(Local.promises) = Memory.bot)
+    :
+      forget_statelocal (st, lc1) (st, lc2)
+  .
+
+
+  Require Import MemoryProps.
+
+
+concrete_promised
+
+Inductive sim_statelocal:
+  sigT (@Language.state ProgramEvent.t) * Local.t -> sigT (@Language.state ProgramEvent.t) * Local.t -> Prop :=
+| forget_statelocal_intro
+    st lc1 lc2
+    (TVIEW : TView.le lc1.(Local.tview) lc2.(Local.tview))
+    (PROMS : lc1.(Local.promises) = Memory.bot)
+  :
+    forget_statelocal (st, lc1) (st, lc2)
+.
+
+
+View.
+
+Inductive forget_memory P msrc mtgt : Prop :=
+| forget_memory_intro
+    (COMPLETE: forall l t (NPROMS: ~ P l t),
+        Memory.get l t msrc = Memory.get l t mtgt)
+    (FORGET: forall l t (PROMS: P l t), Memory.get l t msrc = None)
+.
+
+
+option
+option_rel Message.le
+
+
+Inductive forget_memory P msrc mtgt : Prop :=
+| forget_memory_intro
+    (COMPLETE: forall l t (NPROMS: ~ P l t),
+        Memory.get l t msrc = Memory.get l t mtgt)
+    (FORGET: forall l t (PROMS: P l t), Memory.get l t msrc = None)
+.
+
+
+
+low view
+shorter
+
+
+
+Module Inv.
+
+  Record t mem lang (st: Language.state lang) lc
+         (proms: Memory.t)
+         (spaces : Loc.t -> Time.t -> Prop)
+         (updates : Loc.t -> Time.t -> Prop)
+         (aupdates : Loc.t -> Time.t -> Prop)
+         (mlast: Memory.t): Prop :=
+    {
+      SPACES: forall loc ts (IN: spaces loc ts), concrete_covered proms mem loc ts;
+      AUPDATES: forall loc ts (IN: aupdates loc ts),
+          exists to msg,
+            (<<TS: Time.lt ts to>>) /\
+            (<<GET: Memory.get loc to proms = Some (ts, msg)>>);
+      PROMS: forall
+          loc to m sc (PROM : concrete_promised proms loc to)
+          (FUTURE: unchanged_on spaces mlast m)
+          (UNCHANGED: not_attatched (updates \2/ aupdates) m),
+          exists st' lc' sc' m',
+            (<<STEPS : rtc (tau (@AThread.program_step _))
+                           (Thread.mk _ st lc sc m)
+                           (Thread.mk _ st' lc' sc' m')>>) /\
+            (<<WRITING : is_writing _ st' loc Ordering.relaxed>>);
+      UPDATE : forall
+          loc to m sc (UPD : updates loc to)
+          (FUTURE: unchanged_on spaces mlast m)
+          (UNCHANGED: not_attatched (updates \2/ aupdates) m),
+          exists st' lc' sc' m',
+            (<<STEPS : rtc (tau (@AThread.program_step _))
+                           (Thread.mk _ st lc sc m)
+                           (Thread.mk _ st' lc' sc' m')>>) /\
+            (<<READING : is_updating _ st' loc Ordering.strong_relaxed>>);
+      AUPDATE : forall
+          loc to m sc (UPD : aupdates loc to)
+          (FUTURE: unchanged_on spaces mlast m)
+          (UNCHANGED: not_attatched (updates \2/ aupdates) m),
+          exists st' lc' sc' m',
+            (<<STEPS : rtc (tau (@AThread.program_step _))
+                           (Thread.mk _ st lc sc m)
+                           (Thread.mk _ st' lc' sc' m')>>) /\
+            (<<READING : is_updating _ st' loc Ordering.seqcst>>);
+    }.
+
+End Inv.
+
+
+
+Section SIMPF.
+
+  Inductive thread_wf lang (th: Thread.t lang): Prop :=
+  | thread_wf_intro
+      (SC: Memory.closed_timemap th.(Thread.sc) th.(Thread.memory))
+      (CLOSED: Memory.closed th.(Thread.memory))
+      (LCWF: Local.wf th.(Thread.local) th.(Thread.memory))
+  .
+
+  Inductive sim_pf_one
+            (tid: Ident.t)
+            (mlast: Memory.t)
+            (spaces : (Loc.t -> Time.t -> Prop))
+            (updates: (Loc.t -> Time.t -> Prop))
+            (aupdates: (Loc.t -> Time.t -> Prop))
+            (c_src c_tgt: Configuration.t) : Prop :=
+  | sim_pf_one_intro
+      (FUTURE: unchanged_on spaces mlast c_src.(Configuration.memory))
+      (NOATTATCH: not_attatched (updates \2/ aupdates) c_src.(Configuration.memory))
+      (INV:
+         forall
+           lang_src st_src lc_src lang_tgt st_tgt lc_tgt
+           (TIDSRC: IdentMap.find tid c_src.(Configuration.threads) =
+                    Some (existT _ lang_src st_src, lc_src))
+           (TIDTGT: IdentMap.find tid c_tgt.(Configuration.threads) =
+                    Some (existT _ lang_tgt st_tgt, lc_tgt)),
+           Inv.t c_tgt.(Configuration.memory) _ st_src lc_src lc_tgt.(Local.promises) spaces updates aupdates mlast)
+      (INVBOT:
+         forall
+           (TIDSRC: IdentMap.find tid c_src.(Configuration.threads) = None),
+           (<<SPACESBOT: spaces <2= bot2>>) /\
+           (<<UPDATESBOT: updates <2= bot2>>) /\
+           (<<AUPDATESBOT: aupdates <2= bot2>>))
+  .
+
+  Inductive sim_pf
+            (idents: Ident.t -> Prop)
+            (mlast: Ident.t -> Memory.t)
+            (spaces : Ident.t -> (Loc.t -> Time.t -> Prop))
+            (updates: Ident.t -> (Loc.t -> Time.t -> Prop))
+            (aupdates: Ident.t -> (Loc.t -> Time.t -> Prop))
+            (c_src c_tgt: Configuration.t) : Prop :=
+  | sim_pf_intro
+      (FORGET: forget_config c_src c_tgt)
+      (THREADS: forall tid (IDENT: idents tid),
+          sim_pf_one tid (mlast tid) (spaces tid) (updates tid) (aupdates tid) c_src c_tgt)
+      (RACEFREE: pf_racefree APFConfiguration.step c_src)
+      (WFSRC: Configuration.wf c_src)
+      (WFTGT: Configuration.wf c_tgt)
+      (RESERVEWF: memory_reserve_wf c_tgt.(Configuration.memory))
+      (RESERVERTGT: reserver_exists c_tgt)
+      (RESERVERSRC: reserver_exists c_src)
+  .
+
+  Definition sim_pf_minus_one
+             (tid: Ident.t)
+             (mlast: Ident.t -> Memory.t)
+             (spaces : Ident.t -> (Loc.t -> Time.t -> Prop))
+             (updates: Ident.t -> (Loc.t -> Time.t -> Prop))
+             (aupdates: Ident.t -> (Loc.t -> Time.t -> Prop))
+             (c_src c_tgt: Configuration.t) : Prop :=
+    sim_pf (fun tid' => tid <> tid') mlast spaces updates aupdates c_src c_tgt.
+
+  Inductive sim_pf_all c_src c_tgt: Prop :=
+  | sim_pf_all_intro mlast spaces updates aupdates
+                     (SIM : sim_pf (fun _ => True) mlast spaces updates aupdates c_src c_tgt)
+  .
+
+  Lemma init_pf s tid st lc
+        (TID: IdentMap.find tid (Threads.init s) = Some (st, lc))
+    :
+      Local.promises lc = Memory.bot.
+  Proof.
+    unfold Threads.init in *. erewrite IdentMap.Properties.F.map_o in *.
+    unfold option_map in *. des_ifs.
+  Qed.
+
+  Lemma sim_pf_init
+        s
+        (RACEFREE: pf_racefree APFConfiguration.step (Configuration.init s))
+    :
+      sim_pf_all (Configuration.init s) (Configuration.init s)
+  .
+  Proof.
+    econs.
+    instantiate (1:=fun _ _ _ => False).
+    instantiate (1:=fun _ _ _ => False).
+    instantiate (1:=fun _ _ _ => False).
+    instantiate (1:=fun _ => Memory.init).
+    econs; eauto; ss; i.
+    - econs; i; ss.
+      + unfold Threads.init in *. erewrite IdentMap.Properties.F.map_o in *.
+        unfold option_map in *. des_ifs.
+      + econs.
+        * instantiate (1:= Memory.init). econs; ss; eauto.
+          ii. inv PROMS. ss.
+          exploit init_pf; eauto. i. rewrite x0 in *.
+          inv PROMISED. rewrite Memory.bot_get in *. clarify.
+        * refl.
+    - econs; ss.
+      + refl.
+      + ii. des; clarify.
+      + i. econs; eauto; ii; clarify.
+        exploit init_pf; try apply TIDTGT; eauto. i.
+        rewrite x0 in *. inv PROM.
+        rewrite Memory.bot_get in *. clarify.
+      + i; splits; i; clarify.
+    - eapply Configuration.init_wf.
+    - eapply Configuration.init_wf.
+    - ii. unfold Memory.get in GET. rewrite Cell.init_get in GET.
+      des_ifs.
+    - ii. unfold Memory.get in RESERVE. rewrite Cell.init_get in RESERVE.
+      des_ifs.
+    - ii. unfold Memory.get in RESERVE. rewrite Cell.init_get in RESERVE.
+      des_ifs.
+  Qed.
+
+  Lemma sim_pf_src_no_promise idents mlast spaces updates aupdates c_src c_tgt
+        (SIM: sim_pf idents mlast spaces updates aupdates c_src c_tgt)
+        tid st lc
+        (TIDSRC: IdentMap.find tid c_src.(Configuration.threads) =
+                 Some (st, lc))
+    :
+      lc.(Local.promises) = Memory.bot.
+  Proof.
+    inv SIM. inv FORGET. specialize (THS tid).
+    unfold option_rel in THS. des_ifs. inv THS. auto.
+  Qed.
+
+  Lemma sim_pf_src_no_reserve idents mlast spaces updates aupdates c_src c_tgt
+        (SIM: sim_pf idents mlast spaces updates aupdates c_src c_tgt)
+        loc to from
+        (RESERVE: Memory.get loc to c_src.(Configuration.memory) = Some (from, Message.reserve))
+    :
+      False.
+  Proof.
+    dup SIM. inv SIM. eapply RESERVERSRC in RESERVE; eauto.
+    des. eapply sim_pf_src_no_promise in TIDSRC; eauto.
+    rewrite TIDSRC in *. erewrite Memory.bot_get in *; clarify.
+  Qed.
+
+  Lemma less_covered_max_ts mem0 mem1
+        (INHABITED: Memory.inhabited mem0)
+        (SHORTER: forall loc to (COVER: covered loc to mem0), covered loc to mem1)
+        loc
+    :
+      Time.le (Memory.max_ts loc mem0) (Memory.max_ts loc mem1).
+  Proof.
+    specialize (INHABITED loc). eapply Memory.max_ts_spec in INHABITED.
+    des. dup GET. eapply memory_get_ts_strong in GET. des; clarify.
+    - erewrite GET1. eapply Time.bot_spec.
+    - exploit SHORTER.
+      { econs; eauto. econs; [|refl]. eauto. }
+      intros COVER. inv COVER. inv ITV.
+      eapply Memory.max_ts_spec in GET. des. ss.
+      etrans; eauto.
+  Qed.
+
+  Lemma sim_pf_max_timemap idents mlast spaces updates aupdates c_src c_tgt max
+        (SIM: sim_pf idents mlast spaces updates aupdates c_src c_tgt)
+        (MAX: Memory.max_concrete_timemap c_tgt.(Configuration.memory) max)
+    :
+      TimeMap.le (Memory.max_timemap c_src.(Configuration.memory)) max.
+  Proof.
+    inv SIM. inv WFTGT. inv MEM. inv WFSRC. inv MEM. inv FORGET. ii.
+    inv MEM. inv SHORTER. eapply less_covered_max_ts in COVER; eauto. etrans; eauto.
+    exploit Memory.max_ts_spec.
+    { inv FORGET. erewrite COMPLETE0.
+      - eapply (INHABITED loc).
+      - ii. inv H. destruct st as [lang st]. inv PROMISED. destruct msg.
+        inv WF. exploit THREADS0; eauto. intros []. erewrite BOT in GET. clarify. }
+    i. des. eapply forget_memory_get in GET; eauto. des. destruct msg.
+    - eapply Memory.max_concrete_ts_spec in GET0; eauto. des. auto.
+    - exfalso. eapply NOT.
+      eapply RESERVERTGT in GET0. des. destruct st as [lang st].
+      econs; eauto. econs; eauto.
+  Qed.
+
+  Lemma pf_sim_memory_exists_or_blank L mem_src mem_tgt
+        (MEM: pf_sim_memory L mem_src mem_tgt)
+        loc to from val released
+        (GET: Memory.get loc to mem_tgt = Some (from, Message.concrete val released))
+    :
+      (exists from', (<<GET: Memory.get loc to mem_src = Some (from', Message.concrete val released)>>)) \/
+      (<<BLANK: forall ts (ITV: Interval.mem (from, to) ts),
+          (<<NCOVER: ~ covered loc ts mem_src>>) /\ (<<FORGET: L loc to>>)>>).
+  Proof.
+    inv MEM. dup FORGET. inv FORGET. destruct (classic (L loc to)).
+    - right. ii. split; auto. ii.
+      inv SHORTER. eapply COVER in H0. inv H0.
+      eapply forget_memory_get in GET0; eauto. des; clarify.
+      exploit Memory.get_disjoint.
+      { eapply GET1. }
+      { eapply GET. }
+      i. des; clarify. eapply x0; eauto.
+    - left. erewrite <- COMPLETE in GET; eauto.
+      inv SHORTER. eapply COMPLETE0 in GET. des. eauto.
+  Qed.
+
+
+End SIMPF.
